@prefix : <http://purl.org/lis590OD/Fall17/CrimeChargeOnt#> .
@prefix dc: <http://purl.org/dc/elements/1.1/> .
@prefix tl: <http://purl.org/NET/c4dm/timeline.owl#> .
@prefix dbp: <http://dbpedia.org/resource/> .
@prefix geo: <http://www.w3.org/2003/01/geo/wgs84_pos#> .
@prefix org: <http://www.w3.org/ns/org#> .
@prefix owl: <http://www.w3.org/2002/07/owl#> .
@prefix rdf: <http://www.w3.org/1999/02/22-rdf-syntax-ns#> .
@prefix xml: <http://www.w3.org/XML/1998/namespace> .
@prefix xsd: <http://www.w3.org/2001/XMLSchema#> .
@prefix xsp: <http://www.owl-ontologies.com/2005/08/07/xsp.owl#> .
@prefix doco: <https://svn.code.sf.net/p/sempublishing/code/DoCO/doco.owl> .
@prefix foaf: <http://xmlns.com/foaf/0.1/> .
@prefix prov: <http://www.w3.org/ns/prov#> .
@prefix rdfs: <http://www.w3.org/2000/01/rdf-schema#> .
@prefix skos: <http://www.w3.org/2004/02/skos/core#> .
@prefix swrl: <http://www.w3.org/2003/11/swrl#> .
@prefix wped: <http://en.wikipedia.org/wiki/> .
@prefix dolce: <http://ontology.ip.rm.cnr.it/ontologies/DOLCE-Lite#> .
@prefix event: <http://purl.org/NET/c4dm/event.owl#> .
@prefix swrlb: <http://www.w3.org/2003/11/swrlb#> .
@prefix orgrel: <http://purl.org/lis590od/Fall17/OrgRel> .
@prefix dcterms: <http://purl.org/dc/terms/> .
@prefix protege: <http://protege.stanford.edu/plugins/owl/protege#> .
@prefix lkifnorm: <http://www.estrellaproject.org/lkif-core/norm.owl#> .
@prefix lkifmereo: <http://www.estrellaproject.org/lkif-core/mereology.owl#> .
@prefix lkiflaction: <http://www.estrellaproject.org/lkif-core/action.owl#> .
@prefix lkiflegalrole: <http://www.estrellaproject.org/lkif-core/legal-role.owl#> .
@prefix lkifexpression: <http://www.estrellaproject.org/lkif-core/expression.owl#> .
@base <http://purl.org/lis590OD/Fall17/CrimeChargeOnt> .

<http://purl.org/lis590OD/Fall17/CrimeChargeOnt> rdf:type owl:Ontology .

#################################################################
#    Object Properties
#################################################################

###  http://purl.org/lis590OD/Fall17/CrimeChargeOnt#charges
:charges rdf:type owl:ObjectProperty ;
         owl:inverseOf :isChargedBy ;
         rdfs:domain lkiflegalrole:Professional_Legal_Role ;
         rdfs:range foaf:Person ;
         rdfs:comment "A legal agent can have the ability to charge an offender with a crime."@en .


###  http://purl.org/lis590OD/Fall17/CrimeChargeOnt#createdBy
:createdBy rdf:type owl:ObjectProperty ;
           owl:inverseOf :creates ;
           rdfs:domain lkifnorm:Legal_Document ;
           rdfs:range lkiflegalrole:Professional_Legal_Role ;
           owl:propertyChainAxiom ( [ owl:inverseOf :hasArtifact
                                    ]
                                    :hasActor
                                  ) ;
           rdfs:comment "Links an author/creator of a document to the document the person has created."@en .


###  http://purl.org/lis590OD/Fall17/CrimeChargeOnt#creates
:creates rdf:type owl:ObjectProperty ;
         rdfs:domain lkiflegalrole:Professional_Legal_Role ;
         rdfs:range lkifnorm:Legal_Document .


###  http://purl.org/lis590OD/Fall17/CrimeChargeOnt#hasActor
:hasActor rdf:type owl:ObjectProperty ;
          owl:inverseOf lkiflaction:actor .


###  http://purl.org/lis590OD/Fall17/CrimeChargeOnt#hasArtifact
:hasArtifact rdf:type owl:ObjectProperty ;
             rdfs:domain lkiflaction:Action ;
             rdfs:range lkifnorm:Legal_Document ;
             rdfs:comment "Connects an action with the physical artifact that is produced in the course of the action."@en ;
             rdfs:label "recordedIn"@en .


###  http://purl.org/lis590OD/Fall17/CrimeChargeOnt#hasClassification
:hasClassification rdf:type owl:ObjectProperty ;
                   rdfs:domain lkifnorm:Statute ;
                   rdfs:range :CrimeClassification .


###  http://purl.org/lis590OD/Fall17/CrimeChargeOnt#hasLawViolation
:hasLawViolation rdf:type owl:ObjectProperty ;
                 owl:inverseOf :lawViolationIn ;
                 rdfs:domain :Charge ;
                 rdfs:range lkifnorm:Statute .


###  http://purl.org/lis590OD/Fall17/CrimeChargeOnt#hasRecipient
:hasRecipient rdf:type owl:ObjectProperty ;
              owl:inverseOf :receives ;
              rdfs:domain lkiflaction:Action ;
              rdfs:range foaf:Person .


###  http://purl.org/lis590OD/Fall17/CrimeChargeOnt#isChargedBy
:isChargedBy rdf:type owl:ObjectProperty ;
             rdfs:domain foaf:Person ;
             rdfs:range lkiflegalrole:Professional_Legal_Role .


###  http://purl.org/lis590OD/Fall17/CrimeChargeOnt#isChargedWith
:isChargedWith rdf:type owl:ObjectProperty ;
               rdfs:domain :ChargedPerson ;
               owl:propertyChainAxiom ( :isChargedWith
                                        :hasClassification
                                      ) ,
                                      ( :isChargedWith
                                        <http://www.essepuntato.it/2008/12/pattern#contains>
                                      ) ,
                                      ( :receives
                                        :hasLawViolation
                                      ) .


###  http://purl.org/lis590OD/Fall17/CrimeChargeOnt#isSupportedBy
:isSupportedBy rdf:type owl:ObjectProperty ;
               owl:inverseOf :supports ;
               rdfs:domain lkiflaction:Artifact ;
               rdfs:range lkifexpression:Evidence .


###  http://purl.org/lis590OD/Fall17/CrimeChargeOnt#lawViolationIn
:lawViolationIn rdf:type owl:ObjectProperty .


###  http://purl.org/lis590OD/Fall17/CrimeChargeOnt#receives
:receives rdf:type owl:ObjectProperty ;
          rdfs:domain :ChargedPerson ;
          rdfs:range lkiflaction:Action .


###  http://purl.org/lis590OD/Fall17/CrimeChargeOnt#supports
:supports rdf:type owl:ObjectProperty ;
          rdfs:domain lkifexpression:Evidence ;
          rdfs:range lkiflaction:Artifact ;
          rdfs:comment "Links a charging document with the legal evidence mentioned in the document."@en .


###  http://www.essepuntato.it/2008/12/pattern#contains
<http://www.essepuntato.it/2008/12/pattern#contains> rdf:type owl:ObjectProperty ;
                                                     owl:inverseOf <http://www.essepuntato.it/2008/12/pattern#isContainedBy> ;
                                                     rdfs:domain lkifnorm:Statute ;
                                                     rdfs:range :Statute_Information ;
                                                     rdfs:comment "Refers to a particular section within a document. Not necessarily part-whole relationship."@en .


###  http://www.essepuntato.it/2008/12/pattern#isContainedBy
<http://www.essepuntato.it/2008/12/pattern#isContainedBy> rdf:type owl:ObjectProperty ;
                                                          rdfs:label "isContainedIn"@en .


###  http://www.estrellaproject.org/lkif-core/action.owl#actor
lkiflaction:actor rdf:type owl:ObjectProperty ;
                  rdfs:domain lkiflegalrole:Professional_Legal_Role ;
                  rdfs:range lkiflaction:Action ;
                  rdfs:comment "Specifies that some participant is an actor in the action."@en ;
                  rdfs:label "isActorIn"@en .


###  http://www.estrellaproject.org/lkif-core/mereology.owl#part
lkifmereo:part rdf:type owl:ObjectProperty ;
               owl:inverseOf lkifmereo:part_of ;
               rdfs:label "hasPart"@en .


###  http://www.estrellaproject.org/lkif-core/mereology.owl#part_of
lkifmereo:part_of rdf:type owl:ObjectProperty ;
                  rdfs:domain lkifnorm:Legal_Document ;
                  rdfs:range lkifnorm:Legal_Document ;
                  rdfs:comment "From LKIF: Transitive part-of relation"@en .


###  http://xmlns.com/foaf/0.1/topic
foaf:topic rdf:type owl:ObjectProperty ;
           rdfs:domain lkifnorm:Legal_Document ;
           rdfs:range owl:Thing ;
           owl:propertyChainAxiom ( [ owl:inverseOf :hasArtifact
                                    ]
                                    :hasLawViolation
                                  ) ,
                                  ( [ owl:inverseOf :hasArtifact
                                    ]
                                    :hasRecipient
                                  ) ;
           rdfs:comment "Connects a legal document with any significant content within the document."@en ;
           rdfs:label "hasTopic"@en .


#################################################################
#    Classes
#################################################################

###  http://purl.org/lis590OD/Fall17/CrimeChargeOnt#ArrestingCharge
:ArrestingCharge rdf:type owl:Class ;
                 rdfs:subClassOf :Charge ,
                                 [ rdf:type owl:Restriction ;
                                   owl:onProperty :hasActor ;
                                   owl:allValuesFrom :ArrestingOfficer
                                 ] ;
                 rdfs:comment "A charge action made at the time of an arrest by the arresting officer. Written down in a police report or other record during booking."@en .


###  http://purl.org/lis590OD/Fall17/CrimeChargeOnt#ArrestingOfficer
:ArrestingOfficer rdf:type owl:Class ;
                  rdfs:subClassOf lkiflegalrole:Professional_Legal_Role ;
                  rdfs:comment "An arresting officer is the police department representative who makes an arrest."@en .


###  http://purl.org/lis590OD/Fall17/CrimeChargeOnt#Charge
:Charge rdf:type owl:Class ;
        rdfs:subClassOf lkiflaction:Action ,
                        [ rdf:type owl:Restriction ;
                          owl:onProperty :hasArtifact ;
                          owl:someValuesFrom lkiflaction:Artifact
                        ] ,
                        [ rdf:type owl:Restriction ;
                          owl:onProperty :hasLawViolation ;
                          owl:someValuesFrom lkifnorm:Statute
                        ] ,
                        [ rdf:type owl:Restriction ;
                          owl:onProperty :hasActor ;
                          owl:maxQualifiedCardinality "1"^^xsd:nonNegativeInteger ;
                          owl:onClass lkiflegalrole:Professional_Legal_Role
                        ] ,
                        [ rdf:type owl:Restriction ;
                          owl:onProperty :hasRecipient ;
                          owl:maxQualifiedCardinality "1"^^xsd:nonNegativeInteger ;
                          owl:onClass :ChargedPerson
                        ] ;
        rdfs:comment "An accusation of crime."@en .


###  http://purl.org/lis590OD/Fall17/CrimeChargeOnt#ChargedPerson
:ChargedPerson rdf:type owl:Class ;
               rdfs:subClassOf foaf:Person ,
                               [ rdf:type owl:Restriction ;
                                 owl:onProperty :isChargedBy ;
                                 owl:someValuesFrom lkiflegalrole:Professional_Legal_Role
                               ] ,
                               [ rdf:type owl:Restriction ;
                                 owl:onProperty :isChargedWith ;
                                 owl:someValuesFrom lkifnorm:Statute
                               ] ,
                               [ rdf:type owl:Restriction ;
                                 owl:onProperty :receives ;
                                 owl:someValuesFrom :Charge
                               ] ;
               rdfs:comment "A person who is being charged by a legal agent."@en .


###  http://purl.org/lis590OD/Fall17/CrimeChargeOnt#Complaint
:Complaint rdf:type owl:Class ;
           rdfs:subClassOf lkiflaction:Artifact ,
                           [ rdf:type owl:Restriction ;
                             owl:onProperty :createdBy ;
                             owl:allValuesFrom :Prosecutor
                           ] .


###  http://purl.org/lis590OD/Fall17/CrimeChargeOnt#ConvictingCharge
:ConvictingCharge rdf:type owl:Class ;
                  rdfs:subClassOf :Charge ,
                                  [ rdf:type owl:Restriction ;
                                    owl:onProperty :hasActor ;
                                    owl:allValuesFrom :Judge
                                  ] ;
                  rdfs:comment "A charge action made at the time of a conviction by a judge."@en .


###  http://purl.org/lis590OD/Fall17/CrimeChargeOnt#CrimeClassification
:CrimeClassification rdf:type owl:Class ;
                     rdfs:subClassOf :Statute_Information ;
                     rdfs:comment "Categorization of crimes into misdemeanors, felonies, infractions, and wobblers."@en .


###  http://purl.org/lis590OD/Fall17/CrimeChargeOnt#CrimeCode
:CrimeCode rdf:type owl:Class ;
           rdfs:subClassOf :Statute_Information ,
                           [ rdf:type owl:Restriction ;
                             owl:onProperty lkifmereo:part_of ;
                             owl:someValuesFrom lkifnorm:Statute
                           ] ;
           rdfs:comment "A crime code is the criminal charge in a written form, typically the section title of a statute"@en .


###  http://purl.org/lis590OD/Fall17/CrimeChargeOnt#CriminalRecord
:CriminalRecord rdf:type owl:Class ;
                rdfs:subClassOf lkifnorm:Legal_Document .


###  http://purl.org/lis590OD/Fall17/CrimeChargeOnt#FormalCharge
:FormalCharge rdf:type owl:Class ;
              rdfs:subClassOf :Charge ,
                              [ rdf:type owl:Restriction ;
                                owl:onProperty :hasActor ;
                                owl:allValuesFrom :Prosecutor
                              ] ;
              rdfs:comment "A charge action made to start the proceedings of a criminal case. Written on a charging document typically by a prosecutor."@en .


###  http://purl.org/lis590OD/Fall17/CrimeChargeOnt#Indictment
:Indictment rdf:type owl:Class ;
            rdfs:subClassOf lkiflaction:Artifact ,
                            [ rdf:type owl:Restriction ;
                              owl:onProperty :createdBy ;
                              owl:allValuesFrom :Prosecutor
                            ] .


###  http://purl.org/lis590OD/Fall17/CrimeChargeOnt#Information
:Information rdf:type owl:Class ;
             rdfs:subClassOf lkiflaction:Artifact ,
                             [ rdf:type owl:Restriction ;
                               owl:onProperty :createdBy ;
                               owl:allValuesFrom :Prosecutor
                             ] .


###  http://purl.org/lis590OD/Fall17/CrimeChargeOnt#Judge
:Judge rdf:type owl:Class ;
       rdfs:subClassOf lkiflegalrole:Professional_Legal_Role ;
       rdfs:comment "From NOLO: An official with the authority and responsibility to preside in a court, try lawsuits, and make legal rulings."@en .


###  http://purl.org/lis590OD/Fall17/CrimeChargeOnt#PoliceReport
:PoliceReport rdf:type owl:Class ;
              rdfs:subClassOf lkiflaction:Artifact ,
                              [ rdf:type owl:Restriction ;
                                owl:onProperty :createdBy ;
                                owl:allValuesFrom :ArrestingOfficer
                              ] ;
              rdfs:comment "A police report is a document prepared by a police department representative after an alleged crime has occured. A report can contain information such as the location and date/time of the event, the offender and victim involved, any property impact, and the charge that was allegedly violated."@en .


###  http://purl.org/lis590OD/Fall17/CrimeChargeOnt#Prosecutor
:Prosecutor rdf:type owl:Class ;
            rdfs:subClassOf lkiflegalrole:Professional_Legal_Role ;
            rdfs:comment "From NOLO: A lawyer who works for the local, state, or federal government to bring and litigate criminal cases."@en .


###  http://purl.org/lis590OD/Fall17/CrimeChargeOnt#Statute_Information
:Statute_Information rdf:type owl:Class ;
                     rdfs:comment "Indicates sections within a statute. Not technically legal documents in and of themselves."@en .


###  http://www.estrellaproject.org/lkif-core/action.owl#Action
lkiflaction:Action rdf:type owl:Class ;
                   rdfs:comment "From LKIF: An action is a change which is brought about by a single agent, playing a role. The agent is the holder of some indended outcome of the action: an action is always intentional. The intention of the agent has usually corresponds with an expectation the intended outcome to be brought about: the agent believes in some expectation. Note that the intention might not correspond with the *actual* outcome of the action."@en ;
                   rdfs:label "Legal Action"@en .


###  http://www.estrellaproject.org/lkif-core/action.owl#Artifact
lkiflaction:Artifact rdf:type owl:Class ;
                     rdfs:subClassOf lkifnorm:Legal_Document ,
                                     [ rdf:type owl:Restriction ;
                                       owl:onProperty :isSupportedBy ;
                                       owl:someValuesFrom lkifexpression:Evidence
                                     ] ;
                     rdfs:comment """From LKIF: A physical object created by some person to fulfil a particular purpose.

For this ontology, a charging artifact is always some sort of legal document/record that is generated when a charge is made."""@en ;
                     rdfs:label "Charge Artifact"@en .


###  http://www.estrellaproject.org/lkif-core/expression.owl#Evidence
lkifexpression:Evidence rdf:type owl:Class ;
                        rdfs:subClassOf [ rdf:type owl:Restriction ;
                                          owl:onProperty :supports ;
                                          owl:someValuesFrom lkiflaction:Artifact
                                        ] ;
                        rdfs:comment "From LKIF: Observation and/or statement, used as a backing for a belief."@en ;
                        rdfs:label "Legal Evidence"@en .


###  http://www.estrellaproject.org/lkif-core/legal-role.owl#Professional_Legal_Role
lkiflegalrole:Professional_Legal_Role rdf:type owl:Class ;
                                      rdfs:comment "From LKIF: A professional legal role is a legal profession of some person, examples: lawyer, judge etc."@en ;
                                      rdfs:label "Legal Agent"@en .


###  http://www.estrellaproject.org/lkif-core/norm.owl#Code
lkifnorm:Code rdf:type owl:Class ;
              rdfs:subClassOf lkifnorm:Legal_Document ,
                              [ rdf:type owl:Restriction ;
                                owl:onProperty lkifmereo:part ;
                                owl:someValuesFrom lkifnorm:Statute
                              ] ;
              rdfs:comment "A code is a collection of statutes and laws organized in some fashion, such as by subject."@en .


###  http://www.estrellaproject.org/lkif-core/norm.owl#Legal_Document
lkifnorm:Legal_Document rdf:type owl:Class ;
                        rdfs:subClassOf [ rdf:type owl:Restriction ;
                                          owl:onProperty :createdBy ;
                                          owl:someValuesFrom lkiflegalrole:Professional_Legal_Role
                                        ] ;
                        rdfs:comment "From LKIF: A subclass of a legal source."@en ,
                                     "The legality of a document is most likely related to the fact that a person of the law or legislative body prepared it for some legal purpose."@en .


###  http://www.estrellaproject.org/lkif-core/norm.owl#Statute
lkifnorm:Statute rdf:type owl:Class ;
                 rdfs:subClassOf lkifnorm:Legal_Document ,
                                 [ rdf:type owl:Restriction ;
                                   owl:onProperty <http://www.essepuntato.it/2008/12/pattern#contains> ;
                                   owl:qualifiedCardinality "1"^^xsd:nonNegativeInteger ;
                                   owl:onClass :CrimeClassification
                                 ] ,
                                 [ rdf:type owl:Restriction ;
                                   owl:onProperty <http://www.essepuntato.it/2008/12/pattern#contains> ;
                                   owl:qualifiedCardinality "1"^^xsd:nonNegativeInteger ;
                                   owl:onClass :CrimeCode
                                 ] ;
                 rdfs:comment "A statute is a formal written enactment of a legislative authority that governs a state, city or country. From LKIF: A statute bears one or more norms, all of which are uttered by some legal person. It cannot bear expressions which are uttered by a different kind of agent."@en .


###  http://xmlns.com/foaf/0.1/Person
foaf:Person rdf:type owl:Class ;
            rdfs:comment "A person."@en .


#################################################################
#    Individuals
#################################################################

###  http://purl.org/lis590OD/Fall17/CrimeChargeOnt#Complaint_of_John_Doe
:Complaint_of_John_Doe rdf:type owl:NamedIndividual ,
                                lkiflaction:Artifact .


###  http://purl.org/lis590OD/Fall17/CrimeChargeOnt#Criminal_Damage_to_Property
:Criminal_Damage_to_Property rdf:type owl:NamedIndividual ,
                                      :CrimeCode .


###  http://purl.org/lis590OD/Fall17/CrimeChargeOnt#Felony
:Felony rdf:type owl:NamedIndividual ,
                 :CrimeClassification .


###  http://purl.org/lis590OD/Fall17/CrimeChargeOnt#Formal_Charge_of_John_Doe
:Formal_Charge_of_John_Doe rdf:type owl:NamedIndividual ,
                                    :Charge ;
                           :hasArtifact :Complaint_of_John_Doe ;
                           :hasLawViolation <http://purl.org/lis590OD/Fall17/CrimeChargeOnt#720-5/16-1> ;
                           :hasRecipient :John_Doe ;
                           rdfs:comment "Test instance"@en .


###  http://purl.org/lis590OD/Fall17/CrimeChargeOnt#Illinois_Compiled_Statutes
:Illinois_Compiled_Statutes rdf:type owl:NamedIndividual ,
                                     lkifnorm:Code ;
                            lkifmereo:part <http://purl.org/lis590OD/Fall17/CrimeChargeOnt#720-5/16-1> .


###  http://purl.org/lis590OD/Fall17/CrimeChargeOnt#Infraction
:Infraction rdf:type owl:NamedIndividual ,
                     :CrimeClassification .


###  http://purl.org/lis590OD/Fall17/CrimeChargeOnt#John_Doe
:John_Doe rdf:type owl:NamedIndividual ,
                   foaf:Person .


###  http://purl.org/lis590OD/Fall17/CrimeChargeOnt#Misdemeanor
:Misdemeanor rdf:type owl:NamedIndividual ,
                      :CrimeClassification .


###  http://purl.org/lis590OD/Fall17/CrimeChargeOnt#Sherry_Wong
:Sherry_Wong rdf:type owl:NamedIndividual ,
                      :Prosecutor ,
                      lkiflegalrole:Professional_Legal_Role ;
             lkiflaction:actor :Formal_Charge_of_John_Doe .


###  http://purl.org/lis590OD/Fall17/CrimeChargeOnt#Wobbler
:Wobbler rdf:type owl:NamedIndividual ,
                  :CrimeClassification ;
         rdfs:comment "Classification of a statute that can be either a felony or misdemeanor."@en .


###  http://purl.org/lis590OD/Fall17/CrimeChargeOnt#720-5/16-1
<http://purl.org/lis590OD/Fall17/CrimeChargeOnt#720-5/16-1> rdf:type owl:NamedIndividual ,
                                                                     lkifnorm:Statute ;
                                                            :hasClassification :Wobbler ;
                                                            <http://www.essepuntato.it/2008/12/pattern#contains> :Criminal_Damage_to_Property .


###  Generated by the OWL API (version 4.2.8.20170104-2310) https://github.com/owlcs/owlapi
